Finish embedding of congress contract (for now..)

src/Congress.v
@@ -14,16 +14,24 @@ Definition TxOut := nat.
 Definition ProposalId := nat.
 Definition Chain := nat.
 
+Module AddressSet := MSetAVL.Make Address.as_modern_OT.
+Module NatKeyedMap := FMapAVL.Make OrderedTypeEx.Nat_as_OT.
+Module AddressKeyedMap := FMapAVL.Make Address.as_old_OT.
+
 Record Proposal :=
   {
     txs : list TxOut ;
-    votes : list (address * Z) ;
+    votes : AddressKeyedMap.t Z ;
     voteResult : Z ;
     proposedIn : block_id
   }.
 
-Module AddressSet := MSetAVL.Make Address.as_modern_OT.
-Module NatKeyedMap := FMapAVL.Make OrderedTypeEx.Nat_as_OT.
+Instance etaProposal : Settable _ :=
+  mkSettable
+    ((constructor Build_Proposal) <*> txs
+                                  <*> votes
+                                  <*> voteResult
+                                  <*> proposedIn)%set.
 
 Record Rules :=
   {
@@ -73,7 +81,7 @@ Definition validateRules (rules : Rules) : bool :=
         && (rules.(marginNeededPermille) >=? 0)%Z
         && (rules.(marginNeededPermille) <=? 1000)%Z
         && (rules.(debatingPeriodInBlocks) >=? 0)%Z.
-  
+
 
 Definition init (chain : Chain) (details : contract_call_details) (setup : Setup) : option State :=
   if validateRules setup.(setupRules) then
@@ -88,11 +96,73 @@ Definition init (chain : Chain) (details : contract_call_details) (setup : Setup
 Definition addProposal (txs : list TxOut) (chain : Chain) (state : State) : State :=
   let id := state.(nextProposalId) in
   let proposal := {| txs := txs ;
-                     votes := [] ;
+                     votes := AddressKeyedMap.empty _ ;
                      voteResult := 0 ;
-                     proposedIn := 0 |} in
+                     proposedIn := 0 |} in (* todo: fixme *)
   let newProposals := NatKeyedMap.add id proposal state.(proposals) in
   state[proposals := newProposals][nextProposalId := id + 1].
+
+Local Definition option_bind {A B : Type} (f : A -> option B) (v : option A) : option B :=
+  match v with
+  | Some val => f val
+  | None => None
+  end.
+
+Local Notation "'do' X <- A ; B" := (option_bind (fun X => B) A)
+                                      (at level 200, X ident, A at level 100, B at level 200).
+
+Local Notation unit := Some.
+
+Definition voteProposal
+           (voter : address)
+           (pid : ProposalId)
+           (vote : Z)
+           (state : State)
+  : option State :=
+  do proposal <- NatKeyedMap.find pid state.(proposals) ;
+  let oldVote := match AddressKeyedMap.find voter proposal.(votes) with
+                 | Some oldVote => oldVote
+                 | None => 0%Z
+                 end in
+  let newVotes := AddressKeyedMap.add voter vote proposal.(votes) in
+  let newVoteResult := (proposal.(voteResult) - oldVote + vote)%Z in
+  let newProposal := proposal[votes := newVotes][voteResult := newVoteResult] in
+  unit (set proposals (NatKeyedMap.add pid newProposal) state).
+
+Definition retractVote
+           (voter : address)
+           (pid : ProposalId)
+           (state : State)
+  : option State :=
+  do proposal <- NatKeyedMap.find pid state.(proposals) ;
+  do oldVote <- AddressKeyedMap.find voter proposal.(votes) ;
+  let newVotes := AddressKeyedMap.remove voter proposal.(votes) in
+  let newVoteResult := (proposal.(voteResult) - oldVote)%Z in
+  let newProposal := proposal[votes := newVotes][voteResult := newVoteResult] in
+  unit (set proposals (NatKeyedMap.add pid newProposal) state).
+
+Definition finishProposal
+           (pid : ProposalId)
+           (state : State)
+           (chain : Chain)
+  : option (State * list TxOut) :=
+  do proposal <- NatKeyedMap.find pid state.(proposals) ;
+  let rules := state.(stateRules) in
+  let debateEnd := ((Z.of_nat proposal.(proposedIn)) + rules.(debatingPeriodInBlocks))%Z in
+  let curBlock := 0%Z in (* todo: fixme *)
+  if (curBlock <? debateEnd)%Z then
+    None
+  else
+    let newState := set proposals (NatKeyedMap.remove pid) state in
+    let totalVotesForProposal := Z.of_nat (AddressKeyedMap.cardinal proposal.(votes)) in
+    let totalMembers := Z.of_nat (AddressSet.cardinal state.(members)) in
+    let ayeVotes := ((proposal.(voteResult) + totalVotesForProposal) / 2)%Z in
+    let voteCountPermille := (totalVotesForProposal * 1000 / totalMembers)%Z in
+    let ayePermille := (ayeVotes * 1000 / totalVotesForProposal)%Z in
+    let enoughVoters : bool := (voteCountPermille >=? rules.(minVoteCountPermille))%Z in
+    let enoughAyes : bool := (ayePermille >=? rules.(marginNeededPermille))%Z in
+    let responseTxs := if (enoughVoters && enoughAyes)%bool then proposal.(txs) else [] in
+    unit (newState, responseTxs).
 
 Definition receive
            (chain : Chain)
@@ -103,6 +173,7 @@ Definition receive
   let sender := details.(from) in
   let isFromOwner := sender =? state.(owner) in
   let isFromMember := AddressSet.mem sender state.(members) in
+  let withoutTxs := option_map (fun newState => (newState, [])) in
   match isFromOwner, isFromMember, maybeMsg with
   | true, _, Some (TransferOwnership newOwner) =>
         Some (state[owner := newOwner], [])
@@ -124,303 +195,20 @@ Definition receive
   | _, true, Some (CreateProposal txs) =>
         Some (addProposal txs chain state, [])
 
+  | _, true, Some (VoteForProposal id) =>
+        withoutTxs (voteProposal sender id 1 state)
+
+  | _, true, Some (VoteAgainstProposal id) =>
+        withoutTxs (voteProposal sender id (-1) state)
+                              
+  | _, true, Some (RetractVote id) =>
+        withoutTxs (retractVote sender id state)
+
+  | _, _, Some (FinishProposal id) =>
+        finishProposal id state chain
+
   | _, _, _ =>
         None
     
   end.
                                        
-
-(*
-module Congress exposing (Msg(..), Proposal, ProposalId, Rules, Setup, State, init, receive, version)
-
-{-| Implements a congress contract. This is based on an example contract of the same name
-in Ethereum. This is essentially a simpler version of the DAO contract that was exploited
-in 2016.
-
-The congress allows its members to vote on proposals. A proposal is a transaction that
-will be sent to a specified address if the proposal passes. That means the members of
-the congress vote on how the funds are used by the congress.
-
-Initially the creator of the contract is the owner of the congress. The owner has the
-capability to add or remove members of the congress but they can also transfer ownership
-of the congress to someone else.
-
-The transaction in the proposal can be any arbitrary transaction, including calls to
-other contracts. This makes some very interesting interactions possible. For instance,
-the congress can be set as its own owner and then members can be added or removed only
-by vote, or the rules (like margin required for a proposal to pass) can be changed only
-by vote.
-
--}
-
-import Blockchain2 as Blockchain exposing (Address, Amount, BlockId, Chain, SerializedMsg, Tx, TxOut, Version)
-import Dict exposing (Dict)
-import Set exposing (Set)
-
-
-type alias ProposalId =
-    Int
-
-
-type alias Proposal =
-    { -- Transactions to make if this proposal succeeds
-      txs : List TxOut
-
-    -- What are the votes?
-    , votes : Dict Address Int
-
-    -- Vote result (aye = +1, nay = -1)
-    , voteResult : Int
-
-    -- When was this proposal made?
-    , proposedIn : BlockId
-    }
-
-
-type alias Rules =
-    { -- Minimum permille of participating members for a vote to succeed.
-      -- For instance, if 500, then at least 50% of the members must participate
-      -- in a vote on a proposal for it to succeed.
-      minVoteCountPermille : Int
-
-    -- What is the required permille of ayes / total (500 = 50%)
-    , marginNeededPermille : Int
-
-    -- Number of blocks to debate a proposal
-    , debatingPeriodInBlocks : Int
-    }
-
-
-type alias Setup =
-    { rules : Rules }
-
-
-type Msg
-    = TransferOwnership Address
-    | ChangeRules Rules
-    | AddMember Address
-    | RemoveMember Address
-    | CreateProposal (List TxOut)
-    | VoteForProposal ProposalId
-    | VoteAgainstProposal ProposalId
-    | RetractVote ProposalId
-    | FinishProposal ProposalId
-
-
-type alias State =
-    { owner : Address
-    , rules : Rules
-    , proposals : Dict ProposalId Proposal
-    , nextProposalId : ProposalId
-    , members : Set Address
-    }
-
-
-version : Version
-version =
-    1
-
-
-init : Setup -> Chain -> Tx -> Maybe State
-init { rules } chain tx =
-    if validateRules rules then
-        Just
-            { owner = tx.from
-            , rules = rules
-            , proposals = Dict.empty
-            , nextProposalId = 1
-            , members = Set.empty
-            }
-
-    else
-        Nothing
-
-
-validateRules : Rules -> Bool
-validateRules rules =
-    (rules.minVoteCountPermille >= 0)
-        && (rules.minVoteCountPermille <= 1000)
-        && (rules.marginNeededPermille >= 0)
-        && (rules.marginNeededPermille <= 1000)
-        && (rules.debatingPeriodInBlocks > 0)
-
-
-receive : Chain -> State -> Tx -> Maybe Msg -> Maybe ( State, List TxOut )
-receive chain state tx maybeMsg =
-    let
-        sender =
-            tx.from
-
-        isFromOwner =
-            sender == state.owner
-
-        isFromMember =
-            Set.member sender state.members
-
-        withoutTxs =
-            Maybe.map (\s -> ( s, [] ))
-    in
-    case ( isFromOwner, isFromMember, maybeMsg ) of
-        ( True, _, Just (TransferOwnership newOwner) ) ->
-            Just ( { state | owner = newOwner }, [] )
-
-        ( True, _, Just (ChangeRules newRules) ) ->
-            if validateRules newRules then
-                Just ( { state | rules = newRules }, [] )
-
-            else
-                Nothing
-
-        ( True, _, Just (AddMember member) ) ->
-            Just ( { state | members = Set.insert member state.members }, [] )
-
-        ( True, _, Just (RemoveMember member) ) ->
-            Just ( { state | members = Set.remove member state.members }, [] )
-
-        ( _, True, Just (CreateProposal txs) ) ->
-            Just ( addProposal txs chain state, [] )
-
-        ( _, True, Just (VoteForProposal id) ) ->
-            voteProposal sender id 1 state |> withoutTxs
-
-        ( _, True, Just (VoteAgainstProposal id) ) ->
-            voteProposal sender id -1 state |> withoutTxs
-
-        ( _, True, Just (RetractVote id) ) ->
-            retractVote sender id state |> withoutTxs
-
-        ( _, _, Just (FinishProposal id) ) ->
-            finishProposal id state chain
-
-        _ ->
-            Nothing
-
-
-addProposal : List TxOut -> Chain -> State -> State
-addProposal proposalTxs chain state =
-    let
-        id =
-            state.nextProposalId
-
-        headBlock =
-            Blockchain.headBlock chain
-
-        proposal =
-            { txs = proposalTxs
-            , votes = Dict.empty
-            , voteResult = 0
-            , proposedIn = headBlock.header.blockNumber
-            }
-    in
-    { state
-        | proposals = Dict.insert id proposal state.proposals
-        , nextProposalId = id + 1
-    }
-
-
-voteProposal : Address -> ProposalId -> Int -> State -> Maybe State
-voteProposal voter id vote state =
-    case Dict.get id state.proposals of
-        Nothing ->
-            Nothing
-
-        Just proposal ->
-            let
-                addVote diff =
-                    let
-                        newProposal =
-                            { proposal
-                                | votes = Dict.insert voter vote proposal.votes
-                                , voteResult = proposal.voteResult + diff
-                            }
-
-                        newState =
-                            { state | proposals = Dict.insert id newProposal state.proposals }
-                    in
-                    Just newState
-            in
-            case Dict.get voter proposal.votes of
-                Nothing ->
-                    addVote vote
-
-                Just oldVote ->
-                    addVote (vote - oldVote)
-
-
-retractVote : Address -> ProposalId -> State -> Maybe State
-retractVote voter id state =
-    case Dict.get id state.proposals of
-        Nothing ->
-            Nothing
-
-        Just proposal ->
-            case Dict.get voter proposal.votes of
-                Nothing ->
-                    Nothing
-
-                Just oldVote ->
-                    let
-                        newProposal =
-                            { proposal
-                                | votes = Dict.remove voter proposal.votes
-                                , voteResult = proposal.voteResult - oldVote
-                            }
-
-                        newState =
-                            { state | proposals = Dict.insert id newProposal state.proposals }
-                    in
-                    Just newState
-
-
-finishProposal : ProposalId -> State -> Chain -> Maybe ( State, List TxOut )
-finishProposal id ({ rules, proposals, members } as state) chain =
-    case Dict.get id proposals of
-        Nothing ->
-            Nothing
-
-        Just proposal ->
-            let
-                headBlock =
-                    Blockchain.headBlock chain
-
-                debateEnd =
-                    proposal.proposedIn + rules.debatingPeriodInBlocks
-            in
-            if headBlock.header.blockNumber < debateEnd then
-                Nothing
-
-            else
-                let
-                    newState =
-                        { state | proposals = Dict.remove id proposals }
-
-                    totalVotesForProposal =
-                        Dict.size proposal.votes
-
-                    totalMembers =
-                        Set.size members
-
-                    -- ayes - nays = voteResult
-                    -- ayes + nays = totalVotesForProposal
-                    -- => 2ayes = votesResult + totalVotes
-                    ayeVotes =
-                        (proposal.voteResult + totalVotesForProposal) // 2
-
-                    voteCountPermille =
-                        totalVotesForProposal * 1000 // totalMembers
-
-                    ayePermille =
-                        ayeVotes * 1000 // totalVotesForProposal
-
-                    responseTxs =
-                        if
-                            (voteCountPermille >= rules.minVoteCountPermille)
-                                && (ayePermille >= rules.marginNeededPermille)
-                        then
-                            proposal.txs
-
-                        else
-                            []
-                in
-                Just ( newState, responseTxs )
-*)
